ironfleet/src/Dafny/Distributed/Protocol/RSL/LivenessProof/Seqno.i.dfy
@@ -31,6 +31,7 @@ import opened CommonProof__Requests_i
 import opened Temporal__Heuristics_i
 import opened Temporal__Rules_i
 import opened Temporal__Temporal_s
+import opened AppStateMachine_i
 import opened Environment_s
 import opened EnvironmentSynchrony_s
 
@@ -579,6 +580,7 @@ lemma lemma_RequestNeverHitsInReplyCache(
   requires inp.src == asp.persistent_request.client
   requires inp.msg.RslMessage_Request?
   requires inp.msg.seqno_req == asp.persistent_request.seqno
+  requires inp.msg.val == asp.persistent_request.request
   requires processing_sync_start <= i
   requires PacketProcessingSynchronous(b, asp, processing_sync_start, processing_bound)
   requires LReplicaNextProcessRequest(b[i].replicas[idx].replica, b[i+1].replicas[idx].replica, inp, ExtractSentPacketsFromIos(ios))
@@ -588,6 +590,7 @@ lemma lemma_RequestNeverHitsInReplyCache(
   var executor := b[i].replicas[idx].replica.executor;
   var reply_cache := executor.reply_cache;
   var sent_packets := ExtractSentPacketsFromIos(ios);
+  assert AppValidRequest(inp.msg.val);
   if inp.src in reply_cache && reply_cache[inp.src].Reply? && inp.msg.seqno_req <= reply_cache[inp.src].seqno
   {
     lemma_SequenceNumberReplyCacheInvHolds(b, asp, i, idx);
