ironfleet/src/Dafny/Distributed/Services/RSL/AppStateMachine.s.dfy
@@ -7,7 +7,8 @@ import opened Native__Io_s
 type AppState
 type AppMessage 
 
-function AppInitialize() : AppState 
+function AppInitialize() : AppState
+predicate AppValidRequest(request:AppMessage)
 function AppHandleRequest(m:AppState, request:AppMessage) : (AppState, AppMessage)
 
 function MarshallAppMessage(m:AppMessage) : seq<byte>
